implementations/ne_list.v
@@ -156,9 +156,9 @@ Fixpoint zip {A B: Type} (l: ne_list A) (m: ne_list B): ne_list (A * B) :=
 
     Global Notation ne_list := ne_list.
 
-    Global Notation "[: x ]" := (one x) : nel_scope.
+    Global Notation "[: x :]" := (one x) : nel_scope.
 
-    Global Notation "[: x ; .. ; y ; z ]"
+    Global Notation "[: x ; .. ; y ; z :]"
         := (cons x .. (cons y (one z)) ..) : nel_scope.
 
     Global Infix ":::" := cons (at level 60, right associativity) : nel_scope.
